Model of the queue, join, spawn, and started writing workers

pulse/share/steel/examples/pulse/parallel/Domains.fst
@@ -4,31 +4,342 @@ open Pulse.Main
 open Pulse.Steel.Wrapper
 open Steel.Effect.Common
 
+module R = Steel.ST.Reference
+module HR = Steel.ST.HigherReference
+
 assume val domain : a:Type0 -> (a -> vprop) -> Type0
+// should contain (at least):
+// 1. the reference where we will put the result
+// 2. a lock that gives back the postcondition
 
 assume val joinable :
   #a:Type0 -> #post:(a -> vprop) ->
   domain a post -> vprop
 
-assume val spawn :
+open Steel.Memory
+open Steel.ST.Effect
+open Steel.ST.Util
+
+module Lock = Steel.ST.SpinLock
+
+let unit_emp_stt_pure_pure a p
+  = unit -> stt a emp (fun x -> pure (p x))
+
+let maybe_sat #a (p: a -> prop) (x: option a)
+  = match x with
+  | None -> True
+  | Some x -> p x
+
+// TODO: Once it is possible, we should have an SL pre and post
+let task_elem = (
+  a: Type0 // return type of the computation
+  & p: (a -> prop) // postcondition about the return value
+  & (unit_emp_stt_pure_pure a p) // the computation
+  & r: R.ref (option a) // the reference where we put the result of the computation
+  & Lock.lock (exists_ (fun v -> R.pts_to r full_perm v `star` pure (maybe_sat p v)))
+)
+
+let task_queue: Type u#1 = list task_elem
+
+unfold
+let inv_task_queue
+  (q: HR.ref task_queue) // the task queue
+  (c: R.ref nat) // a counter of how many tasks are currently being performed
+  : vprop
+= (exists_ (fun vq -> exists_ (fun vc ->
+    HR.pts_to q full_perm vq `star`
+    R.pts_to c full_perm vc)))
+
+let create_task_elem #a p f r l: task_elem
+  = (| a, p, f, r, l |)
+
+assume
+val higher_alloc (#a:Type) (x:a)
+  : stt (HR.ref a) emp (fun r -> HR.pts_to r full_perm x)
+//= admit()
+//= (fun _ -> let x = HR.alloc x in return x)
+
+assume
+val higher_read (#a:Type)
+         (#p:perm)
+         (#v:Ghost.erased a)
+         (r:HR.ref a)
+  : stt a
+      (HR.pts_to r p v)
+      (fun x -> HR.pts_to r p v `star` pure (x == Ghost.reveal v))
+      //(requires true)
+//      (ensures fun x -> x == Ghost.reveal v)
+
+assume val higher_write (#a:Type)
+          (#v:Ghost.erased a)
+          (r:HR.ref a)
+          (x:a)
+  : stt unit
+      (HR.pts_to r full_perm v)
+      (fun _ -> HR.pts_to r full_perm x)
+
+
+let enqueue (t: task_elem) (q: task_queue): task_queue
+  = t::q
+
+```pulse
+fn acquire_queue_lock
+  (#q: HR.ref task_queue) (#c: R.ref nat)
+  (l: Lock.lock (inv_task_queue q c))
+  requires emp
+  ensures (exists vq vc. HR.pts_to q full_perm vq ** R.pts_to c full_perm vc)
+{
+  acquire l;
+  rewrite (inv_task_queue q c) as (exists vq vc. HR.pts_to q full_perm vq ** R.pts_to c full_perm vc);
+  ()
+}
+```
+
+```pulse
+fn release_queue_lock
+  (#q: HR.ref task_queue) (#c: R.ref nat)
+  (l: Lock.lock (inv_task_queue q c))
+  requires (exists vq vc. HR.pts_to q full_perm vq ** R.pts_to c full_perm vc)
+  ensures emp
+{
+  rewrite (exists vq vc. HR.pts_to q full_perm vq ** R.pts_to c full_perm vc) as (inv_task_queue q c);
+  release l;
+  ()
+}
+```
+
+let ref_ownership r: vprop
+  = exists_ (fun v -> R.pts_to r full_perm v)
+
+
+let handler #a (post: a -> prop)
+  = (res: R.ref (option a) & Lock.lock (exists_ (fun v -> R.pts_to res full_perm v `star` pure (maybe_sat post v))))
+
+let mk_handler #a (p: a -> prop) (r: R.ref (option a)) (l: Lock.lock (exists_ (fun v -> R.pts_to r full_perm v `star` pure (maybe_sat p v))))
+ : handler p //(res: R.ref (option a) & Lock.lock (exists_ (fun v -> R.pts_to res full_perm v `star` pure (maybe_sat p v))))
+= (| r, l |)
+
+```pulse
+fn spawn_emp
+  (#a:Type0)
+  //(#post : (a -> vprop))
+  (post: (a -> prop))
+  (#q: HR.ref task_queue) (#c: R.ref nat)
+  (l: Lock.lock (inv_task_queue q c))
+  (f : unit_emp_stt_pure_pure a post)
+ requires emp // requires prop?
+ returns r: handler post //(res: R.ref (option a) & Lock.lock (exists_ (fun v -> R.pts_to res full_perm v `star` pure (maybe_sat post v))))
+  //Lock.lock
+ ensures emp
+{
+  let res = alloc #(option a) None;
+  let l_res = new_lock (exists_ (fun v -> R.pts_to res full_perm v `star` pure (maybe_sat post v)));
+  let task = create_task_elem #a post f res l_res;
+
+  //acquire l;
+  //rewrite (inv_task_queue q c) as (exists vq vc. HR.pts_to q full_perm vq ** R.pts_to c full_perm vc);
+  acquire_queue_lock l;
+
+  with vq. assert (HR.pts_to q full_perm vq);
+  let vq = higher_read #_ #full_perm #vq q;
+  higher_write #_ #vq q (enqueue task vq);
+
+  release_queue_lock l;
+
+  let r = mk_handler post res l_res;
+  r
+}
+```
+
+assume val free_ref (#a:Type) (r: R.ref a)
+ //(x:a)
+  : stt unit
+  (exists_ (fun v -> R.pts_to r full_perm v))
+  (fun _ -> emp)
+  
+
+
+```pulse
+fn join
+  (#a:Type0)
+  (#post: (a -> prop))
+  (#q: HR.ref task_queue) (#c: R.ref nat)
+  (l: Lock.lock (inv_task_queue q c))
+  (h: handler post)
+ requires emp
+ returns res: a
+ ensures pure (post res)
+{
+  let r = alloc #(option a) None;
+  while (let res = !r; None? res)
+    invariant b. (exists res. R.pts_to r full_perm res ** pure (b == None? res)
+    ** pure (maybe_sat post res))
+  {
+    acquire h._2;
+    let new_res = !h._1;
+    r := new_res;
+    release h._2;
+    ()
+  };
+  let res = !r;
+  free_ref r;
+  Some?.v res
+}
+```
+
+ 
+
+assume val spawn_model :
  (#a:Type0) -> (#pre : vprop) -> (#post : (a -> vprop)) ->
  ($f : (unit -> stt a pre post)) ->
  stt (domain a post) pre (fun dom -> joinable dom)
 
-assume val join :
+assume val join_model :
   (#a:Type0) -> (#post : (a -> vprop)) ->
   d:domain a post ->
   stt a (joinable d) post
   
 assume val in_parallel_section : vprop
 
-val begin_par_block :
+// invariant on task_queue?
+// monotonocity? can be enforced with a witness token
+// pure post?
+assume val begin_par_block :
   #a:_ -> #pre:_ -> #post:_ ->
   n:nat ->
   (unit -> stt a (in_parallel_section `star` pre) post) ->
   // ^ can maybe take a "blockid" identfying the thread pool?
   // not now at least, since we won't have unscoped sections yet
   stt a pre post
+
+let empty_task_queue: task_queue = []
+
+let inv_queue r: vprop
+ = (exists_ (fun q -> HR.pts_to r full_perm q))
+
+#push-options "--z3rlimit 40"
+
+let len (q: task_queue): nat
+= List.Tot.length q
+
+let rec nth (q: task_queue) (i: nat{i < len q}): task_elem
+= match q with
+| t::q' -> if i = 0 then t else nth q' (i - 1)
+
+assume val assume_prop (p: prop): stt unit emp (fun _ -> pure p)
+
+let get_task (task: task_elem): (a:Type & (unit -> stt a emp (fun _ -> emp)))
+= let (| a, task, _ |) = task in (| a, task |)
+
+assume val replace_elem (q: task_queue) (i: nat) (t: task_elem): task_queue
+
+```pulse
+fn begin_par_block_pulse (#a: Type0)
+  (#pre :vprop) (#post: (a -> vprop))
+  (main_block: (unit -> stt a pre post))
+  requires emp
+  ensures emp
+{
+  let r = higher_alloc empty_task_queue; //([]) in //: R.ref task_queue = magic() in
+  let index_task = alloc 0; // points to the next available task
+  let lock = new_lock (exists_ (fun q -> exists_ (fun i_task ->
+    HR.pts_to r full_perm q `star`
+    R.pts_to index_task full_perm i_task `star`
+    pure (i_task >= 0 /\ available_from q i_task)
+    )));
+  parallel
+    requires (emp) and (emp)
+    ensures (emp) and (emp)
+  {
+    let x = main_block ();
+    () // main thread
+  }
+  {
+    parallel
+      requires (emp) and (emp)
+      ensures (emp) and (emp)
+    {
+      while (true)
+        invariant tr. emp ** pure (tr == true)
+      {
+        acquire lock;
+        let i_task = !index_task;
+        with q. assert (HR.pts_to r full_perm q);
+        let vq = higher_read #_ #full_perm #q r;
+        //let perform_task = i_task < len vq;
+        if (i_task < len vq)
+        {
+          // get the task
+          let task = nth vq i_task;
+          // increase index
+          index_task := i_task + 1;
+
+          assume_prop (available_from vq (i_task + 1));
+          release lock;
+
+          let to_perform = get_task task;
+          let res = (to_perform._2) (); // Actually performing the task
+
+          // Finally, we put the result of the task in the queue
+          let new_task = Mkdtuple3 task._1 task._2 (Done res);
+          acquire lock;
+
+          // Step 2: perform task
+          //let (| a, actual_task, _ |) = task;
+
+
+          release lock;
+          ()
+        }
+        else {
+          release lock;
+          ()
+        }
+      };
+      () // worker
+    }
+    {
+      () // worker
+    };
+    ()
+  };
+  admit()
+}
+```
+
+  (*
+  Code:
+  let q: task_queue = [] in
+  let l = new_lock in
+  parallel (
+    parallel (
+      ...
+    )
+  )
+  (
+    parallel (
+      ...
+    )
+  )
+  *)
+
+ (*
+ let handler: domain a post = spawn (fun () -> ...)
+ consumes precondition
+ returns token
+the precondition goes into the lock for this particular location...
+1) We acquire the *main* lock
+2) We add one task to the shared list
+--> we need to add
+- the actual task (unit -> stt ...)
+- the lock (Lock.lock p, where p is a vprop)
+- some value that says whether the task is
+  1. available
+  2. ongoing
+  3. finished (with result...)
+We allocate a new lock
+ *)
+
 
   // begin_par_block 16 (fun () ->
   //   let th1 = spawn(..) in
